sync

Qualification/Basic.lean
@@ -6,6 +6,28 @@ structure Lts: Type 1 where mk::
   Label: Type
   trans: State → Label → State → Prop
 
+def lts1: Lts := {
+  State := Nat
+  initial := 0
+  Label := String
+  trans s1 l s2 := s2 = s1+1 ∧ l = "inc"
+}
+
+
+def lts2: Lts := {
+  State := String
+  initial := "init"
+  Label := String
+  trans _ l _ := l = "inc"
+}
+
+notation lts " # " s1 " —" l "⟶ " s2 => Lts.trans lts s1 l s2
+
+example: (lts1: Lts) # (6: Nat) — "inc" ⟶ (7: Nat) := sorry
+
+example: lts2 # "init" —"inc"⟶ "cool" :=
+  sorry
+
 structure Model where mk::
   Fluent: Type
   lts: Lts
@@ -24,3 +46,10 @@ def ConModel' (Constant: Type) :=
   }
 
 example: Type 1 := ConModel' String
+
+def Lts.trans_clos (lts: Lts)
+: lts.State → List lts.Label → lts.State → Prop :=
+  ReflTransLab lts.trans
+
+
+notation lts "# " s1 "—" l "⟶⋆" s2 => Lts.trans_clos lts s1 l s2
