Qualification/Utils.lean
@@ -1,5 +1,6 @@
 
-abbrev EndoRel α := α → α → Prop
+abbrev Rel α β := α → β → Prop
+abbrev EndoRel α := Rel α α
 
 inductive ReflTransGen {α} (r: EndoRel α): EndoRel α where
   | refl (x: α): ReflTransGen r x x
@@ -15,3 +16,19 @@ example: ReflTransGen all_nat 0 5 := by
   . exact ReflTransGen.refl 0
   . unfold all_nat
     exact True.intro
+
+
+inductive ReflTransLab {State Label: Type} (r: State → Label → State → Prop)
+: State → List Label → State → Prop where
+  | refl (s: State): ReflTransLab r s [] s
+  | cons (s1 s2 s3: State) (l12: Label) (l23: List Label):
+                   r s1 l12 s2 →
+      ReflTransLab r s2 l23 s3 →
+      ReflTransLab r s1 (l12 :: l23) s3
+
+theorem List.snoc {State Label: Type} {r: State → Label → State → Prop}:
+  ∀ (s1 s2 s3: State) (l12: List Label) (l23: Label),
+      ReflTransLab r s1 l12 s2 →
+                   r s2 l23 s3 →
+      ReflTransLab r s1 (l23 :: l12) s3
+:= by sorry
